# ----- DSD-specific namespaces -----

@prefix bonn-attribute:  <http://data.openbudgets.eu/ontology/dsd/bonn-budget-simplified-updated/attribute/> .
@prefix bonn-dimension:  <http://data.openbudgets.eu/ontology/dsd/bonn-budget-simplified-updated/dimension/> .
@prefix bonn-dsd-slice:  <http://data.openbudgets.eu/ontology/dsd/bonn-budget-simplified-updated/slice/> .

# ----- OpenBudgets.eu namespaces -----

@prefix obeu:             <http://data.openbudgets.eu/ontology/> .
@prefix obeu-attribute:   <http://data.openbudgets.eu/ontology/dsd/attribute/> .
@prefix obeu-dimension:   <http://data.openbudgets.eu/ontology/dsd/dimension/> .
@prefix obeu-measure:     <http://data.openbudgets.eu/ontology/dsd/measure/> .

# ----- Generic namespaces ------

@prefix org:              <http://www.w3.org/ns/org#> .
@prefix qb:               <http://purl.org/linked-data/cube#> .
@prefix rdf:              <http://www.w3.org/1999/02/22-rdf-syntax-ns#> .
@prefix rdfs:             <http://www.w3.org/2000/01/rdf-schema#> .
@prefix skos:             <http://www.w3.org/2004/02/skos/core#> .
@prefix xsd:              <http://www.w3.org/2001/XMLSchema#> .

# ----- DSD -----


<http://data.openbudgets.eu/ontology/dsd/bonn-budget-simplified-updated> a qb:DataStructureDefinition ;
  rdfs:label "Data structure definition for the approved budget of Bonn (Germany)."@en ;  

  qb:component [ qb:dimension obeu-dimension:organization ;
                 qb:componentAttachment qb:DataSet ],
               [ qb:dimension obeu-dimension:operationCharacter],
               [ qb:dimension obeu-dimension:fiscalYear ;
                 qb:componentAttachment qb:DataSet ],
               [ qb:dimension obeu-dimension:budgetPhase ;
                 qb:componentAttachment qb:DataSet ],      
               [ qb:dimension bonn-dimension:economicClassification ],
               [ qb:dimension bonn-dimension:profitCenter ],
               [ qb:dimension bonn-dimension:functionalClassification ],
               [ qb:attribute obeu-attribute:currency ;
                 qb:componentRequired true ;
                 qb:componentAttachment qb:DataSet ],
               [ qb:measure obeu-measure:amount ]  .

bonn-dimension:economicClassification a rdf:Property, qb:CodedProperty, qb:DimensionProperty;
  rdfs:label "Economic Classification"@en ;
  rdfs:comment "Identifies the type of expenditure incurred or source of revenues. The economic classification is organized hierarchical in two levels."@en ;
  rdfs:subPropertyOf obeu-dimension:economicClassification ;
  rdfs:range skos:Concept ;
  qb:codeList <http://data.openbudgets.eu/resource/codelist/kostenartenuebersicht_bonn> ;
  rdfs:isDefinedBy <http://data.openbudgets.eu/ontology/dsd/bonn-budget-simplified-updated>.

 bonn-dimension:profitCenter a rdf:Property, qb:CodedProperty, qb:DimensionProperty;
  rdfs:label "Profit Center (PC) Classification"@en ;
  rdfs:comment "A combination of administrative classification and functional classification. A profitcenter consists of: amt / administrative classification (Digit 2-5) + functional classification (digit 6-9), the whole PC can be used as a subproperty of obeu:administrativeClassification and each PC code has it's own description"@en ;
  rdfs:subPropertyOf bonn-dimension:administrativeClassification ;
  rdfs:range skos:Concept ;
  qb:codeList <http://data.openbudgets.eu/resource/codelist/profitcenter_bonn> ;
  rdfs:isDefinedBy <http://data.openbudgets.eu/ontology/dsd/bonn-budget-simplified-updated>.

 bonn-dimension:functionalClassification a rdf:Property, qb:CodedProperty, qb:DimensionProperty;
  rdfs:label "Functional Classification"@en ;
  rdfs:comment "A functional classification of budget datasets from the City of Bonn"@en ;
  rdfs:subPropertyOf obeu-dimension:functionalClassification ;
  rdfs:range skos:Concept ;
  qb:codeList <http://data.openbudgets.eu/resource/codelist/produktuebersicht_bonn> ;
  rdfs:isDefinedBy <http://data.openbudgets.eu/ontology/dsd/bonn-budget-simplified-updated>.  
 