# ----- DSD-specific namespaces -----

@prefix oc-measure:    <http://data.openbudgets.eu/ontology/dsd/oc-2007-2013/measure/> .
@prefix oc-dimension:  <http://data.openbudgets.eu/ontology/dsd/oc-2007-2013/dimension/> .
@prefix oc-dsd-slice:  <http://data.openbudgets.eu/ontology/dsd/oc-2007-2013/slice/> .

# ----- OpenBudgets.eu namespaces -----

@prefix obeu:             <http://data.openbudgets.eu/ontology/> .
@prefix obeu-attribute:   <http://data.openbudgets.eu/ontology/dsd/attribute/> .
@prefix obeu-dimension:   <http://data.openbudgets.eu/ontology/dsd/dimension/> .
@prefix obeu-measure:     <http://data.openbudgets.eu/ontology/dsd/measure/> .

# ----- Generic namespaces ------

@prefix org:              <http://www.w3.org/ns/org#> .
@prefix qb:               <http://purl.org/linked-data/cube#> .
@prefix rdf:              <http://www.w3.org/1999/02/22-rdf-syntax-ns#> .
@prefix rdfs:             <http://www.w3.org/2000/01/rdf-schema#> .
@prefix skos:             <http://www.w3.org/2004/02/skos/core#> .
@prefix xsd:              <http://www.w3.org/2001/XMLSchema#> .

# ----- DSD -----


<http://data.openbudgets.eu/ontology/dsd/oc-2007-2013> a qb:DataStructureDefinition ;
  rdfs:label "Data structure definition for the Italian Structural and Cohesion Funds beneficiaries between 2007 and 2013, collected by OpenCoesione.it ."@en ;  

  qb:component [ qb:dimension obeu-dimension:organization ;
                 qb:componentAttachment qb:Slice ],
               [ qb:dimension obeu-dimension:partner ;
                 qb:componentAttachment qb:Slice ],
               [ qb:dimension obeu-dimension:date ],
               [ qb:dimension obeu-dimension:operationCharacter;
                 qb:componentAttachment qb:DataSet ],
               [ qb:dimension obeu-dimension:project ;
                 qb:componentAttachment qb:Slice ],
               [ qb:dimension oc-dimension:QSNfunctionalClassification ;
                 qb:componentAttachment qb:Slice ],
               [ qb:dimension oc-dimension:EUfunctionalClassification ;
                 qb:componentAttachment qb:Slice ],
               [ qb:dimension oc-dimension:OCfunctionalClassification ;
                 qb:componentAttachment qb:Slice ],
               [ qb:dimension oc-dimension:OCprogrammeClassification ;
                 qb:componentAttachment qb:Slice ],
               [ qb:dimension oc-dimension:programmeClassification ;
                 qb:componentAttachment qb:Slice ],
               [ qb:dimension oc-dimension:CUPeconomicClassification ;
                 qb:componentAttachment qb:Slice ],
               [ qb:dimension oc-dimension:ATECOeconomicClassification ;
                 qb:componentAttachment qb:Slice ],
               [ qb:dimension oc-dimension:CUPadministrativeClassification ;
                 qb:componentAttachment qb:Slice ],               
               [ qb:attribute obeu-attribute:currency ;
                 qb:componentRequired true ;
                 qb:componentAttachment qb:DataSet ],
               [ qb:attribute obeu-attribute:location ;
                 qb:componentAttachment qb:Slice ],  
               [ qb:measure oc-measure:amountTotal ],
               [ qb:measure oc-measure:amountEU ],
               [ qb:measure oc-measure:amountNational ];
               
  qb:sliceKey  oc-dsd-slice:slice-by-project .


# ----- Slice key definition -----

oc-dsd-slice:slice-by-project a qb:SliceKey ;
	rdfs:label "Slice by project"@en ;
	rdfs:comment "Slice grouping observations of the same project with the different payments as observations."@en ;
	qb:componentProperty obeu-dimension:organization ;
    qb:componentProperty obeu-dimension:partner ;
    qb:componentProperty obeu-dimension:project ;
    qb:componentProperty oc-dimension:QSNfunctionalClassification ;
    qb:componentProperty oc-dimension:EUfunctionalClassification ;
    qb:componentProperty oc-dimension:OCfunctionalClassification ;
    qb:componentProperty oc-dimension:OCprogrammeClassification ;
    qb:componentProperty oc-dimension:programmeClassification ;
    qb:componentProperty oc-dimension:CUPeconomicClassification ;
    qb:componentProperty oc-dimension:ATECOeconomicClassification ;
    qb:componentProperty oc-dimension:CUPadministrativeClassification ;
    qb:componentProperty obeu-attribute:location .
	

# ----- Component properties -----

oc-dimension:QSNfunctionalClassification a rdf:Property, qb:CodedProperty, qb:DimensionProperty;
  rdfs:label "Functional classification according to QSN"@en ;
  rdfs:comment "The functional classification according to QSN (Quadro Strategico Nazionale = National Strategic Framework) is hierarchically structured in three levels, priorities, general objectives, and specific objectives."@en ;
  rdfs:subPropertyOf obeu-dimension:functionalClassification ;
  rdfs:range skos:Concept ;
  qb:codeList <http://data.openbudgets.eu/resource/codelist/qsn-functional-class> ;
  rdfs:isDefinedBy <http://data.openbudgets.eu/ontology/dsd/oc-2007-2013> .
  
 oc-dimension:EUfunctionalClassification a rdf:Property, qb:CodedProperty, qb:DimensionProperty;
  rdfs:label "Functional classification according to EU priorities"@en ;
  rdfs:comment "The EU functional classification is defined by EU Regulation 1828/2006 and provides 86 entries that describe the sectoral categories of expenditure of the projects."@en ;
  rdfs:subPropertyOf obeu-dimension:functionalClassification ;
  rdfs:range skos:Concept ;
  qb:codeList <http://data.openbudgets.eu/resource/codelist/eu-functional-class> ;
  rdfs:isDefinedBy <http://data.openbudgets.eu/ontology/dsd/oc-2007-2013> .
  
oc-dimension:OCfunctionalClassification a rdf:Property, qb:CodedProperty, qb:DimensionProperty;
  rdfs:label "Functional classification according to OpenCoesione"@en ;
  rdfs:comment "The OpenCoesione functional classification defines 13 thematic topics, based on an aggregate of the EU priorities and sectoral classifications in the CUP (Codice Unico di Progetto) system."@en ;
  rdfs:subPropertyOf obeu-dimension:functionalClassification ;
  rdfs:range skos:Concept ;
  qb:codeList <http://data.openbudgets.eu/resource/codelist/oc-functional-class> ;
  rdfs:isDefinedBy <http://data.openbudgets.eu/ontology/dsd/oc-2007-2013> .  
  
oc-dimension:OCprogrammeClassification a rdf:Property, qb:CodedProperty, qb:DimensionProperty;
  rdfs:label "Programme classification"@en ;
  rdfs:comment "The programme classification is hierarchically structured in two levels, funds and programmes."@en ;
  rdfs:subPropertyOf obeu-dimension:programmeClassification ;
  rdfs:range skos:Concept ;
  qb:codeList <http://data.openbudgets.eu/resource/codelist/oc-programme-class-a> ;
  rdfs:isDefinedBy <http://data.openbudgets.eu/ontology/dsd/oc-2007-2013> .    
  
oc-dimension:programmeClassification a rdf:Property, qb:CodedProperty, qb:DimensionProperty;
  rdfs:label "Programme classification"@en ;
  rdfs:comment "For the structural fund, the programmes are hierarchically structured into axes and objectives, for the development and cohesion fund the programmes are hierarchically structured into lines and actions."@en ;
  rdfs:subPropertyOf obeu-dimension:programmeClassification ;
  rdfs:range skos:Concept ;
  qb:codeList <http://data.openbudgets.eu/resource/codelist/oc-programme-class-b> ;
  rdfs:isDefinedBy <http://data.openbudgets.eu/ontology/dsd/oc-2007-2013> .    

oc-dimension:CUPeconomicClassification a rdf:Property, qb:CodedProperty, qb:DimensionProperty;
  rdfs:label "Economic classification according to CUP"@en ;
  rdfs:comment "The CUP (Codice Unico di Progetto) system classifies the projects hierarchically in nature and type."@en ;
  rdfs:subPropertyOf obeu-dimension:economicClassification ;
  rdfs:range skos:Concept ;
  qb:codeList <http://data.openbudgets.eu/resource/codelist/cup-economic-class> ;
  rdfs:isDefinedBy <http://data.openbudgets.eu/ontology/dsd/oc-2007-2013> .  

oc-dimension:ATECOeconomicClassification a rdf:Property, qb:CodedProperty, qb:DimensionProperty;
  rdfs:label "Economic classification according to ATECO"@en ;
  rdfs:comment "ATECO (attivit√† economiche = economic activities) is the national version of the European nomenclature, Nace Rev. 2, published in the Official Journal of 20 December 2006 (Regulation (EC) no 1893/2006 of the European Parliament and of the Council of 20 December 2006). The classification is structrued hierarchically in five levels."@en ;
  rdfs:subPropertyOf obeu-dimension:economicClassification ;
  rdfs:range skos:Concept ;
  qb:codeList <http://data.openbudgets.eu/resource/codelist/ateco-class> ;
  rdfs:isDefinedBy <http://data.openbudgets.eu/ontology/dsd/oc-2007-2013> .  

oc-dimension:CUPadministrativeClassification a rdf:Property, qb:CodedProperty, qb:DimensionProperty;
  rdfs:label "Administrative classification according to CUP"@en ;
  rdfs:comment "The CUP (Codice Unico di Progetto) system classifies the projects hierarchically in sectors, subsectors and categories."@en ;
  rdfs:subPropertyOf obeu-dimension:administrativeClassification ;
  rdfs:range skos:Concept ;
  qb:codeList <http://data.openbudgets.eu/resource/codelist/cup-admin-class> ;
  rdfs:isDefinedBy <http://data.openbudgets.eu/ontology/dsd/oc-2007-2013> .  
  
oc-measure:amountTotal a rdf:Property, qb:MeasureProperty ;
  rdfs:label "Amount Total"@en ;
  rdfs:comment "Total payment of the transaction."@en ;
  rdfs:subPropertyOf obeu-measure:amount ;
  rdfs:isDefinedBy <http://data.openbudgets.eu/ontology/dsd/oc-2007-2013> .    
  
oc-measure:amountEU a rdf:Property, qb:MeasureProperty ;
  rdfs:label "Amount EU"@en ;
  rdfs:comment "Amount paid by the European Union."@en ;
  rdfs:subPropertyOf obeu-measure:amount ;
  rdfs:isDefinedBy <http://data.openbudgets.eu/ontology/dsd/oc-2007-2013> .   
  
oc-measure:amountNational a rdf:Property, qb:MeasureProperty ;
  rdfs:label "Amount National"@en ;
  rdfs:comment "National amount paid by PAC (Piano di Azione per la Coesione = Action Plan for Cohesion)."@en ;
  rdfs:subPropertyOf obeu-measure:amount ;
  rdfs:isDefinedBy <http://data.openbudgets.eu/ontology/dsd/oc-2007-2013> .    
  
